\chapter*{Lecture 15}
\begin{recall}{}{}
\begin{itemize}
\item Reduction of order technique
\begin{itemize}
\item missing terms
\item find second solution
\end{itemize}
\end{itemize}
\end{recall}


\subsubsection*{General procedure}
\begin{enumerate}
\item Introduce $y_2(x)=V(x)y_1(x)$ and compute the first two derivatives
\item Sub the resulting equations into the ODE and for a homogeneous equation, remove the last term on the LHS.
\item Solve for $V(x)$ using the order reduction (method of missing terms)
\item Solve for $y_2$
\item[(5)]Find the general form of the solution: $y=c_1 y_1+c_2y_2$
\end{enumerate}


\begin{center}
\noindent\rule{4cm}{0.4pt}
\end{center}

\begin{exmp}{Order reduction (find second solution):}\\
Solve:
\begin{equation*}
\frac{d^2y}{dx^2}+4\frac{dy}{dx} + 6y=0
\label{originalODE}
\end{equation*}
knowing that $y_1=e^{-3x}$. Find $y_2$.
\clearpage
\textbf{Solution:}
\begin{itemize}
\item[Step 1] Introduce $y_2=Vy_1= Ve^{-3x}$ and compute derivatives:
\begin{equation*}
\frac{dy_2}{dx}=-3 Ve^{-3x}+e^{-3x}\frac{dV}{dx}
\end{equation*}

\begin{equation*}
\frac{d^2y_2}{dx^2}=9 Ve^{-3x} +  e^{-3x}\frac{d^2V}{dx^2}-6e^{-3x}\frac{dV}{dx}
\end{equation*}
We replace in the original ODE \eqref{originalODE}:
\begin{equation*}
\underbrace{9 Ve^{-3x} +  e^{-3x}\frac{d^2V}{dx^2}-6e^{-3x}\frac{dV}{dx}}_{\frac{d^2y}{dx^2}}+4\left(\underbrace{-3 Ve^{-3x}+e^{-3x}\frac{dV}{dx}}_{\frac{dy}{dx}}\right) + 3\underbrace{Ve^{-3x}}_y=0
\end{equation*}

After a number of algebraic simplifications, we end up with:

\begin{equation*}
\boxed{\frac{d^2V}{dx^2}-2\frac{dV}{dx}=0}
\label{tempsODE}
\end{equation*}
\item[Step 3] Solve for $V$. Let $W=\frac{dV}{dx}$  and $\frac{dW}{dx}=\frac{d^2V}{dx^2}$  and sub into \eqref{tempsODE}:
\begin{equation*}
\frac{dW}{dx}-2W=0
\end{equation*}
and solve for $W$:
\begin{equation*}
\int \frac{1}{W}dW=\int2 dx+c_1 \qquad \qquad W=c_1e^{2x}
\end{equation*}
Transform back into $V$:
\begin{equation}
V=\int W dW+c_2=\int c_1 e^{2x}dx +c_2 \qquad \qquad V=c_1e^{2x}+c_2
\end{equation}
\item[Step 4] Solve for $y_2$:
\begin{equation}
y_2 = V(x) y_1 = (c_1e^{2x}+c_2)y_1
\end{equation}

QUESTION: Are the solutions linearly independent????
What if $c_1=0$? The solutions are not-independent!
\item[Step 5] Find the general form of the solution.\\
The general form of the solution of a linear, homogeneous second-order ODE looks like:
\begin{equation*}
y_{general}=Ay_1+By_2
\end{equation*}
We can therefore write our solution as:
\begin{equation*}
y_{general}=Ay_1+B(c_1e^{2x}+c_2)y_1
\end{equation*}
or:
\begin{equation*}
y_{general}=Ay_1+Bc_1e^{2x}y_1+Bc_2y_1 = \underbrace{(A+Bc_2)}_C y_1+\underbrace{Bc_1}_De^{2x}y_1
\end{equation*}
\begin{equation*}
y_{general}=C y_1+De^{2x}y_1 = Cy_1+Dy_2
\end{equation*}
Therefore, $y_1=e^{-3x}$ (given by the problem) and $y_2=e^{2x}y_1=e^{-x}$.
 At this point, it is not a bad idea to check the linear independence of our solution basis:
 \begin{equation*}
W(y_1,y_2)=\left|\begin{bmatrix}
    y_1 & y_2  \\
    y'_1 & y'_2
  \end{bmatrix}\right| = y_1y'_2 -y'_1y_2 
\end{equation*}
 \begin{equation*}
 = e^{-3x}(-e^{-x})-(-3)e^{-3x}e^{-x}=2e^{-4x}\neq 0
 \end{equation*}
 
 $y_1$ and  $y_2$  are linearly independent. So our answer is:
 \begin{equation*}
\boxed{y_{2}=e^{-x}}
\end{equation*}
\end{itemize}

\end{exmp}


\begin{center}
\noindent\rule{4cm}{0.4pt}
\end{center}

\begin{exmp}{Order reduction (find second solution):}\\
Solve:
\begin{equation}
9\frac{d^2y}{dx^2}-6\frac{dy}{dx} + y=0
\end{equation}

knowing $y_1=e^{1/3 x}$ find $y_2$ and $y_{general}$.\\
\textbf{Solution:}
\begin{itemize}
\item[Step 1] Introduce $y_2=Vy_1=Ve^{1/3 x}$:
\begin{equation*}
\frac{dy_2}{dx}=1/3 Ve^{1/3x}+e^{1/3x}\frac{dV}{dx}
\end{equation*}

\begin{equation*}
\frac{d^2y_2}{dx^2}=1/9 Ve^{1/3x} +  e^{1/3x}\frac{d^2V}{dx^2}+2/3 e^{1/3x} \frac{dV}{dx}
\end{equation*}
\item[Step 2] Sub into the ODE:
[Steps on the board]

\item[Step 3] Solve for $V$.
\begin{equation*}
{9\frac{d^2V}{dx^2}=0} \qquad \boxed{\frac{d^2V}{dx^2}=0}
\end{equation*}
or :
\begin{equation*}
V(x)=c_1x+c_2
\end{equation*}
\item[Step 4] Solve for $y_2$:
\begin{equation*}
y_2(x)=Vy_1=(c_1x+c_2)e^{1/3x}
\end{equation*}
\item[Step 5] Find the general form of the solution.\\
\begin{equation*}
y_{general} = Ay_1+By_2=Ae^{1/3x} +B(c_1x+c_2)e^{1/3x}=(A+Bc_2)e^{1/3x}+Bc_1e^{1/3x}
\end{equation*}
This yields:
\begin{equation*}
\boxed{y_2= xy_1 = xe^{1/3x}}
\end{equation*}
Our general solution is:
\begin{equation*}
\boxed{y_{general} = Cy_1+Dy_2=Ce^{1/3x}+Dxe^{1/3x}}
\end{equation*}

Check linear independence! (Wronskian)
\end{itemize}

\end{exmp}


\begin{center}
\noindent\rule{4cm}{0.4pt}
\end{center}



