\chapter*{Lecture 23}
\begin{recall}{}{}
\begin{itemize}
\item Variation of Parameter
\end{itemize}
\end{recall}


Solution procedure for VoP:
\begin{enumerate}
\item Find homogeneous solution
\item Assume a particular solution of the form:
\begin {equation*}
y_p=v_1(x)y_1(x) + v_2(x)y_2(x)
\end {equation*}
\item Set up equations and solve for $v_1$ and $v_2$
\item Assemble the general solution
\item Apply IC (if provided)
\end{enumerate}

\begin{exmp}{VoP:}\\
Solve using variation of parameters:
\begin {equation*}
y''-2y'+y=xe^x
\end {equation*}
with $y(0)=1$ and $y'(0)=0$
(this is a constant coefficient equation)\\

\textbf{Solution}\\
\begin{itemize}
\item Find $y_h$:\\
Aux. Eq: $r^2-2r+1=0$ we have two identical, real roots $r=r_1=r_2=1$. The homogeneous solutions are:
\begin {equation*}
y_1=e^x \qquad y_2=xe^x
\end {equation*}
or 
\begin {equation*}
\boxed{y_h=c_1e^x +c_2 xe^x}
\end {equation*}
\item Assume $y_p=v_1(x)y_1 + v_2(x) y_2=v_1e^x +v_2 xe^x$
\item Set up equations:
\begin {align*}
v'_1y'_1 + v'_2 y'_2=F(x) \qquad &\text{after sub in ODE (recall last class result)}\\
v'_1y_1 + v'_2 y_2=0 \qquad &\text{impose condition}
\end {align*}
We compute the derivatives of the homogeneous solutions:
\begin {align*}
y_1 = e^x \qquad y_2 = xe^x\\
y'_1 = e^x \qquad y'_2 = e^x+xe^x
\end {align*}
this yields:
\begin {align*}
v'_1e^x + v'_2 (e^x+xe^x)=xe^x \qquad \text{after sub in ODE}\\
v'_1e^x + v'_2 xe^x=0 \qquad \text{impose condition}
\end {align*}
after simplification of the exponents, we find:
\begin {align*}
v'_1(x)=-x^2\\
v'_2(x)=x
\end {align*}
After integration, we obtain:
\begin {align*}
v_1(x)=-\frac{x^3}{3}+a\\
v_2(x)=\frac{x^2}{2}+b
\end {align*}
\begin {equation*}
\boxed{y_p=-\frac{x^3}{3}e^x +ae^x +\frac{x^2}{2}xe^x+bxe^x}
\end {equation*}
\item General solution is:
\begin {equation*}
y_g=y_h+y_p=c_1e^x +c_2 xe^x-\frac{x^3}{3}e^x +ae^x +\frac{x^2}{2}xe^x+bxe^x
\end {equation*}
Let $c=c_1+a$ and $d=c_2+b$
\begin {equation*}
\boxed{y_g=ce^x +d xe^x+\frac{x^3}{6}e^x}
\end {equation*}
\item Apply ICs (applied on the GENERAL SOLUTION!)
\begin {equation*}
y_g(0)= ce^0 +d 0e^0+\frac{0^3}{6}e^0=c=1
\end {equation*}
and 
\begin {align*}
y'_g= ce^x  +d e^x+d xe^x+\frac{x^2}{2}e^x+\frac{x^3}{6}e^x\\
y'_g(0)= ce^0  +d e^0+d 0e^0+\frac{0^2}{2}e^0+\frac{0^3}{6}e^0\\
y'_g(0)= c  +d=0 \qquad d=-c=-1
\end {align*}
Final solution:
\begin {equation*}
\boxed{y_g=e^x - xe^x+\frac{x^3}{6}e^x}
\end {equation*}


\end{itemize}


\end{exmp}

\updateinfo[October 30, 2018]

