\chapter*{Lecture 19}
\begin{recall}{}{}
\begin{itemize}
\item Auxiliary equations
\end{itemize}
\end{recall}





\section{Method of Undetermined Coefficients (MUC)}
How do we solve non-homogeneous, linear, constant coefficient  equations? 


A general solution solution of a nonhomogeneous, linear equation is the sum of:
\begin{equation}
\boxed{y_{general}=y_{homogeneous} + y_{particular}}
\end{equation}
where $y_\text{homogeneous}$ corresponds to the homogeneous solution (RHS=0), and the $y_\text{particular}$ corresponds to any particular solution to the nonhomogeneous equation.

We note that, despite the common terminology, a  "particular solution" to a second order ODE is slightly different from the "particular solution" previously defined (defined numerical values of the integrative constants).


%https://www.khanacademy.org/math/differential-equations/second-order-differential-equations/undetermined-coefficients/v/undetermined-coefficients-3

If we have a second-order, linear constant coefficient ODE of the form:
\begin{equation*}
ay''+by'+cy=F(x)
\end{equation*}
The homogenous solution satisfies (can be solved via auxiliary equation, order reduction etc):
\begin{equation*}
ay_h''+by_h'+cy_h=0
\end{equation*}
whereas, the particular solution satisfies:
\begin{equation*}
ay_p''+by_p'+cy_p=F(x)
\end{equation*}

The general solution is the sum of the particular and homogeneous solutions, therefore:
\begin{equation*}
a(y_h''+y_p'')+b(y_h'+y_p')+c(y_h+y_p)=F(x)
\end{equation*}
or:
\begin{equation*}
\underbrace{ay_h''+by_h'+cy_h}_0 + \underbrace{ay_p''+by_p'+cy_p}_{F(x)}=F(x)
\end{equation*}


In other words, the general solution of a second-order, constant-coefficient, nonhomogeneous, linear ODE is:
\begin{equation}
y_{general}=y_{h} + y_{p} = c_1y_1+c_2y_2 + y_p
\end{equation}
In this section, we propose a method to find the particular solution $y_p$.


The Method of Undertermined Coefficient (MUC) is nothing more than a "juditious guess". We will present the method using an example:

\begin{exmp}{MUC:}\\
Solve the following non-homogeneous equation:
\begin{equation}
y''+4y=8x^2
\end{equation}
Solution:\\
We recall that our solution is:
\begin{equation}
y_{g}=y_{h} + y_{p} 
\end{equation}
\begin{itemize}
\item Homogeneous solution:
\textbf{Find} $y_h$\\
\begin{equation}
y_h''+4y_h=0
\end{equation}
Can be solved via auxiliary equation:
\begin{equation}
r^2+4=0
\end{equation}
Since $b^2-4ac<0$, we have two imaginary roots. We define:
\begin{align*}
\alpha=-b/(2a) = 0\ \qquad \beta=\frac{\sqrt{4ac-b^2}}{2a}=\frac{\sqrt{16}}{2}=2\\
\end{align*}
The solutions are:
\begin{align*}
y_1=e^\alpha\cos(\beta x)=cos(2x)\\
y_2=e^\alpha\sin(\beta x)=sin(2x)\\
\end{align*}
The homogeneous solution is then:
\begin{align*}
y_h=C_1 cos(2x)+C_2 sin(2x)\\
\end{align*}
\item Particular solution:
\textbf{Find} $y_p$:\\
We have to find a solution $y_p(x)$ such that the combination $y''+4y$ gives us a function of $x$, namely $8x^2$.\\
We suppose a generic form of the solution to be:
\begin{equation}
y(x)= A_2x^2+A_1x+A_0
\end{equation}
Therefore: $y(x)''= 2A_2$.
By substituting into the ODE, we obtain:
\begin{align*}
2A_2+4(A_2x^2+A_1x+A_0)=8x^2\\
4A_2x^2 +4A_1 x+ (2A_2+4A_0)=8x^2 + 0x + 0\\
\end{align*}
Therefore, we have: $4A_2=8$, $4A_1=0$, and $2A_2+4A_0=0$. Thus $A_2=2$, $A_1=0$ and $A_0=-1$.

Our particular solution is $y_p=2x^2-1$.
\end{itemize}
The general solution is then:
\begin{align*}
y_{general}=y_h+y_p=C_1 cos(2x)+C_2 sin(2x) +2x^2-1\\
\end{align*}
\end{exmp}


\begin{exmp}{MUC:}\\
Solve the following non-homogeneous equation:
\begin{equation*}
y''-3y'-4y=3e^{2x}
\end{equation*}
Solution:\\

\begin{equation}
y_{g}=y_{h} + y_{p} 
\end{equation}
\begin{itemize}
\item Homogeneous solution:
\begin{equation*}
y''-3y'-4y=0
\end{equation*}
Solve with auxiliary equation:
\begin{equation*}
r^2-3r-4= (r-4)(r+1)=0
\end{equation*}
We have two real rool: -1 and 4.\\
The homogeneous solution is:
\begin{align*}
y_h=C_1 e^{4x}+C_2 e^{-x}\\
\end{align*}
\item Particular solution:
We guess that our solution looks something like: $y_p=Ae^{2x}$\\
We compute 
\begin{align*}
y'_p=2Ae^{2x} \qquad y''_p=4Ae^{2x}
\end{align*}
We sub into our ODE:
\begin{equation*}
4Ae^{2x}-3(2Ae^{2x})-4(Ae^{2x})=3e^{2x}
\end{equation*}
To satisfy the equation we have $A=-1/2$!

\end{itemize}
The general solution is then:
\begin{align*}
y_{general}=y_h+y_p=C_1 e^{4x}+C_2 e^{-x} - \frac{e^{2x}}{2}
\end{align*}
\end{exmp}



